src/ReactorModel/Execution/Reactor.lean
@@ -13,6 +13,12 @@ def Action.schedule (a : Action) (t : Time) (v : Value) : Action :=
 def List.targets (cs : List Change) :=
   { t : Reactor.Component.Valued × ID | ∃ c ∈ cs, c.Targets t.fst t.snd }
 
+theorem List.mem_targets_cons (h : c ∈ tl.targets) : c ∈ (hd :: tl).targets := by
+  sorry
+
+theorem List.target_mem_targets {cs : List Change} (hc : c ∈ cs) (ht : c.target = some t) : t ∈ cs.targets := by
+  sorry
+
 namespace ReactorType
 namespace Updatable
 
@@ -44,16 +50,16 @@ theorem equiv_eq_dependencies {rtr₁ : α} (e : rtr₁ ≈ rtr₂) :
 def scheduledTags (rtr : α) : Set Time.Tag := 
   { g | ∃ i a, (rtr[.act][i] = some a) ∧ (g ∈ a.keys) }
 
--- TODO?: Make this handle tag names better.
-scoped macro "change_cases " change:term : tactic => 
-  `(tactic| cases $change:term <;> try cases ‹Change.Normal›; cases ‹Reactor.Component.Valued›)
+scoped macro "cases_change " change:term : tactic => `(tactic| 
+  cases $change:term <;> try cases ‹Change.Normal›; cases ‹Reactor.Component.Valued›; cases ‹Kind›
+)
 
 theorem apply_equiv (rtr : α) (c : Change) : (apply rtr c) ≈ rtr := by
-  change_cases c <;> first | rfl | apply LawfulUpdatable.equiv
+  cases_change c <;> first | rfl | apply LawfulUpdatable.equiv
 
 theorem apply_preserves_unchanged {c : Change} (rtr : α) (h : ¬c.Targets cpt i) :
     (apply rtr c)[cpt][i] = rtr[cpt][i] := by
-  change_cases c <;> first | rfl | exact LawfulUpdatable.obj?_preserved (Change.Targets.norm_not h)
+  cases_change c <;> first | rfl | exact LawfulUpdatable.obj?_preserved (Change.Targets.norm_not h)
 
 variable {rtr : α}
 
@@ -70,6 +76,11 @@ theorem apply_action_change (h : rtr[.act][i] = some a) :
   simp [apply, LawfulUpdatable.obj?_updated]
   exact ⟨_, ⟨h, rfl⟩⟩ 
 
+theorem apply_ne_target_comm (ht : c₁.target ≠ c₂.target ∨ c₁.target = none) : 
+    apply (apply rtr c₁) c₂ = apply (apply rtr c₂) c₁ := by
+  cases_change c₁ <;> cases_change c₂ <;> simp [apply, Change.target] at *
+  all_goals exact LawfulUpdatable.update_ne_comm $ by simp_all
+    
 theorem apply'_equiv (rtr : α) : (cs : List Change) → (apply' rtr cs) ≈ rtr 
   | .nil        => .refl
   | .cons hd tl => Equivalent.trans (apply'_equiv (apply rtr hd) tl) (apply_equiv rtr hd)
@@ -81,9 +92,39 @@ theorem apply'_preserves_unchanged {cs : List Change} {cpt : Reactor.Component.V
     have ⟨hh, ht⟩ := List.all₂_cons _ _ _ |>.mp h
     exact apply_preserves_unchanged rtr hh ▸ hi ht 
 
-theorem apply'_disjoint_targets_comm (hd : Disjoint cs₁.targets cs₂.targets) : 
-    apply' (apply' rtr cs₁) cs₂ = apply' (apply' rtr cs₂) cs₁ :=
-  sorry
+theorem apply'_apply_ne_targets_comm (ht : ∀ {t}, c.target = some t → t ∉ cs.targets) : 
+    apply (apply' rtr cs) c = apply' (apply rtr c) cs := by
+  induction cs generalizing rtr <;> simp [apply'] at *
+  case cons hd tl hi =>
+    suffices h : hd.target ≠ c.target ∨ hd.target = none by 
+      rw [hi $ fun _ _ h hm => ht _ _ h $ List.mem_targets_cons hm, apply_ne_target_comm h]
+    by_contra hc
+    push_neg at hc
+    have ⟨_, h⟩ := Option.ne_none_iff_exists.mp hc.right
+    exact ht _ _ (hc.left ▸ h.symm) $ List.target_mem_targets (by simp) h.symm
 
+theorem apply'_disjoint_targets_comm (ht : Disjoint cs₁.targets cs₂.targets) : 
+    apply' (apply' rtr cs₁) cs₂ = apply' (apply' rtr cs₂) cs₁ := by
+  induction cs₁ generalizing rtr <;> cases cs₂ <;> simp [apply'] at *
+  case cons.cons hd₁ tl₁ hd₂ tl₂ hi =>
+    have h₁ : Disjoint (List.targets tl₁) (List.targets (hd₂ :: tl₂)) := by
+      simp [Set.disjoint_iff_forall_ne]
+      intro _ _ hm₁ _ _ hm₂ h₁ h₂
+      subst h₁ h₂    
+      exact Set.disjoint_left.mp ht (List.mem_targets_cons hm₁) hm₂
+    have h₂ : hd₁.target ≠ hd₂.target ∨ hd₁.target = none := by
+      by_contra hc
+      push_neg at hc
+      have ⟨_, h⟩ := Option.ne_none_iff_exists.mp hc.right
+      have h₁ := (hd₁ :: tl₁).target_mem_targets (by simp) h.symm
+      have h₂ := (hd₂ :: tl₂).target_mem_targets (by simp) (hc.left ▸ h.symm)
+      exact Set.disjoint_left.mp ht h₁ h₂
+    have h₃ : ∀ {t}, hd₁.target = some t → ¬t ∈ tl₂.targets := by
+      intro _ h hm
+      have h₁ := (hd₁ :: tl₁).target_mem_targets (by simp) h
+      exact Set.disjoint_left.mp ht h₁ $ List.mem_targets_cons hm
+    rw [hi h₁, apply_ne_target_comm h₂, ←apply', ←apply', ←apply'_apply_ne_targets_comm h₃]
+    rfl
+    
 end Indexable
 end ReactorType
